tests/CustomIndexing.lean
@@ -1,0 +1,15 @@
+/-
+Copyright (c) 2022 Jannis Limperg. All rights reserved.
+Released under Apache 2.0 license as described in the file LICENSE.
+Authors: Jannis Limperg
+-/
+
+import Aesop
+
+set_option aesop.check.all true
+
+example (h : α) : α := by
+  fail_if_success aesop (rule_sets [-builtin,-default]) (add safe h (apply (index := [target False])))
+  aesop                 (rule_sets [-builtin,-default]) (add safe h apply)
+
+-- See Com test for a more realistic scenario.
